

Schrodinger equation

admin

2025-12-30

1 Schrodinger Equation

A derivation

$$i\hbar \frac{\partial \psi}{\partial t} = -\frac{\hbar^2}{2m} \frac{\partial^2 \psi}{\partial x^2} + V\psi$$

1.1 In 1 dimension

From Einstein, we know that for photons:

$$E = \hbar\omega, \quad p = \hbar k$$

From de Broglie, we know that these are true for other particles as well. QM is linear \implies describing plane waves is sufficient Let's consider a plane wave like:

$$\psi(x, t) = \psi_0 e^{i(kx - \omega t)}$$

Now let's find the energy and momentum operators. We know that:

$$\frac{\partial \psi}{\partial t} = -i\omega\psi, \quad \frac{\partial \psi}{\partial x} = ik\psi$$

So:

$$\frac{\hbar}{-i} \frac{\partial \psi}{\partial t} = E\psi = i\hbar \frac{\partial \psi}{\partial t},$$

$$\frac{\hbar}{i} \frac{\partial \psi}{\partial x} = p\psi = -i\hbar \frac{\partial \psi}{\partial x}$$

From Newton's laws we get that:

$$p = mv \implies K = \frac{1}{2}mv^2 = \frac{p^2}{2m}$$

And since energy is conserved, let's introduce a potential energy operator V , so that the potential energy of our particle is $V\psi$. Then, we get:

$$E = K + V$$

1.2 In 3 dimensions

Now x , p and k are vectors \mathbf{x} , \mathbf{p} and \mathbf{k} . So the plane wave is:

$$\psi(\mathbf{x}, t) = \psi_0 e^{i(\mathbf{k} \cdot \mathbf{x} - \omega t)}$$

The energy doesn't change:

$$\frac{\partial \psi}{\partial t} = -i\omega\psi \implies E\psi = i\hbar \frac{\partial \psi}{\partial t}$$

But the spacial derivative is now the gradient:

$$\nabla \psi = \begin{pmatrix} \frac{\partial}{\partial x} \\ \frac{\partial}{\partial y} \\ \frac{\partial}{\partial z} \end{pmatrix} \psi_0 e^{i(k_x x + k_y y + k_z z - \omega t)} = \begin{pmatrix} ik_x \\ ik_y \\ ik_z \end{pmatrix} \psi = i\mathbf{k}\psi$$

Which leaves us with the momentum:

$$\frac{\hbar}{i} \nabla \psi = \mathbf{p}\psi = -i\hbar \nabla \psi$$

But for the energy we need p^2 , so let's see what happens if we take the next spacial derivative, the divergence (since $\mathbf{p}\psi$ is a vector).

$$\nabla \cdot (\mathbf{p}\psi) = \partial_x(p_x\psi) + \partial_y(p_y\psi) + \partial_z(p_z\psi)$$

Since \mathbf{p} is independent of \mathbf{x} (\mathbf{p} is a constant), we can pull its components from the derivatives:

$$= p_x \partial_x \psi + p_y \partial_y \psi + p_z \partial_z \psi$$

$$= (p_x ik_x + p_y ik_y + p_z ik_z) \psi$$

$$= i(\mathbf{p} \cdot \mathbf{k})\psi = i\hbar(\mathbf{k} \cdot \mathbf{k})\psi = i\hbar k^2\psi$$

$$\implies \frac{\hbar}{i}\nabla \cdot (\mathbf{p}\psi) = p^2\psi = -\hbar^2\nabla^2\psi$$

Now, just like we did in 1D, we can use $K = p^2/2m$ for the conservation of energy and we get the Schrodinger equation in 3d:

$$\boxed{i\hbar\frac{\partial\psi}{\partial t} = -\frac{\hbar^2}{2m}\nabla^2\psi + V\psi}$$